Working on gcr

ConsistentRegions.v
@@ -523,3 +523,259 @@ Proof.
   intros. erewrite gcr_write_t1; eauto. erewrite gcr_write_term; eauto.
 Qed.
 
+(* ------------------------------------------------------------------------- *)
+(* region-exclusivity                                                        *)
+(* ------------------------------------------------------------------------- *)
+
+Definition region_exclusivity (t : tm) := forall ad,
+  (one_init ad t \/ no_init ad t) /\
+  (one_cr   ad t \/ no_cr   ad t) /\
+  (one_init ad t -> no_cr   ad t) /\
+  (one_cr   ad t -> no_init ad t).
+
+(* inversion --------------------------------------------------------------- *)
+
+Local Ltac solve_inv_regexc :=
+  intros * H; try match goal with |- _ /\ _ => split end; intros ad';
+  specialize (H ad') as [[? | ?] [[? | ?] [? ?]]]; repeat split; repeat spec;
+  try inv_oneinit; try inv_onecr; try inv_nocr; try inv_noinit; auto; intros ?;
+  exfalso; eauto using noinit_oneinit_contradiction, nocr_onecr_contradiction. 
+
+Local Lemma inv_regexc_fun : forall x Tx t,
+  region_exclusivity <{fn x Tx t}> ->
+  region_exclusivity t.
+Proof. solve_inv_regexc. Qed.
+
+Local Lemma inv_regexc_call : forall t1 t2,
+  region_exclusivity <{call t1 t2}> ->
+  region_exclusivity t1 /\ region_exclusivity t2.
+Proof. solve_inv_regexc. Qed.
+
+Local Lemma inv_regexc_new : forall t T,
+  region_exclusivity <{new t : T}> ->
+  region_exclusivity t.
+Proof. solve_inv_regexc. Qed.
+
+Local Lemma inv_regexc_init : forall ad t T,
+  region_exclusivity <{init ad t : T}> ->
+  region_exclusivity t.
+Proof. solve_inv_regexc. Qed.
+
+Local Lemma inv_regexc_load : forall t,
+  region_exclusivity <{*t}> ->
+  region_exclusivity t.
+Proof. solve_inv_regexc. Qed.
+
+Local Lemma inv_regexc_asg : forall t1 t2,
+  region_exclusivity <{t1 := t2}> ->
+  region_exclusivity t1 /\ region_exclusivity t2.
+Proof. solve_inv_regexc. Qed.
+
+Local Lemma inv_regexc_acq : forall t1 x t2,
+  region_exclusivity <{acq t1 x t2}> ->
+  region_exclusivity t1 /\ region_exclusivity t2.
+Proof. solve_inv_regexc. Qed.
+
+Local Lemma inv_regexc_cr : forall ad t,
+  region_exclusivity <{cr ad t}> ->
+  region_exclusivity t.
+Proof. solve_inv_regexc. Qed.
+
+Local Lemma inv_regexc_spawn : forall t,
+  region_exclusivity <{spawn t}> ->
+  region_exclusivity t.
+Proof. solve_inv_regexc. Qed.
+
+Ltac invc_regexc :=
+  match goal with
+  | H : region_exclusivity <{unit        }> |- _ => clear H
+  | H : region_exclusivity <{nat _       }> |- _ => clear H
+  | H : region_exclusivity <{var _       }> |- _ => clear H
+  | H : region_exclusivity <{fn _ _ _    }> |- _ => eapply inv_regexc_fun   in H
+  | H : region_exclusivity <{call _ _    }> |- _ => eapply inv_regexc_call  in H
+  | H : region_exclusivity <{& _ : _     }> |- _ => clear H
+  | H : region_exclusivity <{new _ : _   }> |- _ => eapply inv_regexc_new   in H
+  | H : region_exclusivity <{init _ _ : _}> |- _ => eapply inv_regexc_init  in H
+  | H : region_exclusivity <{* _         }> |- _ => eapply inv_regexc_load  in H
+  | H : region_exclusivity <{_ := _      }> |- _ => eapply inv_regexc_asg   in H
+  | H : region_exclusivity <{acq _ _ _   }> |- _ => eapply inv_regexc_acq   in H
+  | H : region_exclusivity <{cr _ _      }> |- _ => eapply inv_regexc_cr    in H
+  | H : region_exclusivity <{spawn _     }> |- _ => eapply inv_regexc_spawn in H
+  end;
+  repeat match goal with
+  | H : region_exclusivity _ /\ region_exclusivity _ |- _ => destruct H
+  end.
+
+(* ------------------------------------------------------------------------- *)
+
+Local Lemma gcr_rewrite_call_t1 : forall t1 t2 R,
+  ~ value t1 ->
+  gcr <{call t1 t2}> R = gcr t1 R.
+Proof.
+  intros * H. simpl. destruct t1; auto; exfalso; auto using value.
+Qed.
+
+Local Lemma gcr_rewrite_call_t2 : forall t1 t2 R,
+  value t1 ->
+  gcr <{call t1 t2}> R = gcr t2 R.
+Proof.
+  intros * H. simpl. destruct t1; auto; invc H.
+Qed.
+
+Local Lemma gcr_rewrite_initX : forall ad t T R,
+  gcr <{init ad t : x&T}> R = gcr t (R_ad ad).
+Proof. trivial. Qed.
+
+Local Lemma gcr_rewrite_initW : forall ad t T R,
+  gcr <{init ad t : w&T}> R = gcr t R.
+Proof. trivial. Qed.
+
+Local Lemma gcr_rewrite_asg_t1 : forall t1 t2 R,
+  ~ value t1 ->
+  gcr <{t1 := t2}> R = gcr t1 R.
+Proof.
+  intros * H. simpl. destruct t1; auto; exfalso; auto using value.
+Qed.
+
+Local Lemma gcr_rewrite_asg_t2 : forall t1 t2 R,
+  value t1 ->
+  gcr <{t1 := t2}> R = gcr t2 R.
+Proof.
+  intros * H. simpl. destruct t1; auto; invc H.
+Qed.
+
+(* gcr (get-current-region) simplification *)
+Ltac kappa :=
+ repeat match goal with
+ | H : context C [ gcr <{call ?t1 ?t2}> ?R ], H' : ~ value ?t1 |- _ =>
+   rewrite (gcr_rewrite_call_t1 t1 t2 R H') in H
+
+ | H : context C [ gcr <{call ?t1 ?t2}> ?R ], H' : value   ?t1 |- _ =>
+   rewrite (gcr_rewrite_call_t2 t1 t2 R H') in H
+
+ | H : context C [ gcr <{?t1 := ?t2}> ?R ], H' : ~ value ?t1 |- _ =>
+   rewrite (gcr_rewrite_asg_t1 t1 t2 R H') in H
+
+ | H : context C [ gcr <{?t1 := ?t2}> ?R ], H' : value   ?t1 |- _ =>
+   rewrite (gcr_rewrite_asg_t2 t1 t2 R H') in H
+
+ | H : context C [gcr <{unit                }> _] |- _ => simpl in H
+ | H : context C [gcr <{nat _               }> _] |- _ => simpl in H
+ | H : context C [gcr <{var _               }> _] |- _ => simpl in H
+ | H : context C [gcr <{fn _ _ _            }> _] |- _ => simpl in H
+ | H : context C [gcr <{call ?t _           }> _] |- _ => destruct (value_dec t)
+ | H : context C [gcr <{& _ : _             }> _] |- _ => simpl in H
+ | H : context C [gcr <{new _ : _           }> _] |- _ => simpl in H
+ | H : context C [gcr <{init _ _ : Unit     }> _] |- _ => simpl in H
+ | H : context C [gcr <{init _ _ : Num      }> _] |- _ => simpl in H
+ | H : context C [gcr <{init _ _ : r&_      }> _] |- _ => simpl in H
+ | H : context C [gcr <{init _ _ : x&_      }> _] |- _ => simpl in H
+ | H : context C [gcr <{init _ _ : w&_      }> _] |- _ => simpl in H
+ | H : context C [gcr <{init _ _ : (_ --> _)}> _] |- _ => simpl in H 
+ | H : context C [gcr <{init _ _ : Safe ?T  }> _] |- _ => destruct T 
+ | H : context C [gcr <{init _ _ : ?T       }> _] |- _ => destruct T 
+ | H : context C [gcr <{* _                 }> _] |- _ => simpl in H
+ | H : context C [gcr <{?t := _             }> _] |- _ => destruct (value_dec t)
+ | H : context C [gcr <{acq _ _ _           }> _] |- _ => simpl in H
+ | H : context C [gcr <{cr _ _              }> _] |- _ => simpl in H
+ | H : context C [gcr <{spawn _             }> _] |- _ => simpl in H
+ end.
+
+Lemma gcr_noinit_nocr_contradiction : forall ad t R,
+  R <> R_ad ad ->
+  gcr t R = R_ad ad ->
+  no_init ad t ->
+  no_cr ad t ->
+  False.
+Proof.
+  intros * ? Hgcr **. gendep R. induction t; intros;
+  invc_noinit; invc_nocr; kappa; auto; invc Hgcr; eauto; do 2 spec;
+  match goal with _ : addr, ad : addr |- _ => eapply (IHt (R_ad ad)) end;
+  trivial; intros F; invc F; eauto.
+Qed.
+
+Corollary gcr_noinit_nocr_contradiction1 : forall tid ad t,
+  gcr t (R_tid tid) = R_ad ad ->
+  no_init ad t ->
+  no_cr ad t ->
+  False.
+Proof.
+  intros. eapply gcr_noinit_nocr_contradiction; eauto. intros F. invc F.
+Qed.
+
+Corollary gcr_noinit_nocr_contradiction2 : forall ad' ad t,
+  gcr t (R_ad ad') = R_ad ad ->
+  ad <> ad' ->
+  no_init ad t ->
+  no_cr ad t ->
+  False.
+Proof.
+  intros. eapply gcr_noinit_nocr_contradiction; eauto. intros F. invc F. auto.
+Qed.
+
+Lemma oneinit_or_onecr_from_gcr : forall ad t tid,
+  region_exclusivity t ->
+  (* --- *)
+  gcr t (R_tid tid) = R_ad ad ->
+  (one_init ad t \/ one_cr ad t).
+Proof.
+  intros * Hregexc Hgcr. assert (Hregexc' := Hregexc).
+  induction t; kappa; invc_regexc; repeat spec; try solve [invc Hgcr];
+  destruct (Hregexc ad) as [[? | ?] [[? | ?] _]]; eauto; invc_noinit; invc_nocr;
+  try solve [exfalso; eauto using gcr_noinit_nocr_contradiction1];
+  match goal with ad1 : addr, ad2 : addr |- _ => nat_eq_dec ad1 ad2 end;
+  exfalso; eauto using gcr_noinit_nocr_contradiction2.
+Qed.
+
+#[export] Hint Extern 8 =>
+  match goal with
+  | |- R_invalid <> R_tid _   => intros F; invc F
+  | |- R_invalid <> R_ad  _   => intros F; invc F
+  | |- R_tid _   <> R_ad  _   => intros F; invc F
+  | |- R_tid _   <> R_invalid => intros F; invc F
+  | |- R_ad _    <> R_invalid => intros F; invc F
+  | |- R_ad _    <> R_tid _   => intros F; invc F
+  end : core.
+
+Lemma gcr_ad_tid_contradiction : forall tid ad t,
+  gcr t (R_ad ad) = R_tid tid ->
+  False.
+Proof.
+  intros * Hgcr. gendep ad.
+  induction t; intros; kappa; eauto; invc Hgcr; auto.
+Qed.
+
+Lemma gcr_tid1_tid2_contradiction : forall tid1 tid2 t,
+  tid1 <> tid2 ->
+  gcr t (R_tid tid1) = R_tid tid2 ->
+  False.
+Proof.
+  intros * ? Hgcr.
+  induction t; intros; kappa; eauto using gcr_ad_tid_contradiction;
+  invc Hgcr; auto.
+Qed.
+
+Lemma gcr_invalid_impossibility  : forall t R,
+  R <> R_invalid ->
+  gcr t R = R_invalid ->
+  False.
+Proof.
+  intros * Hgcr. gendep R.
+  induction t; intros; kappa; eauto; try solve [invc Hgcr; auto];
+  match goal with ad : addr |- _ => eapply (IHt (R_ad ad)); eauto end.
+Qed.
+
+Corollary gcr_tid_invalid_contradiction : forall tid t,
+  gcr t (R_tid tid) = R_invalid ->
+  False.
+Proof.
+  intros. eapply (gcr_invalid_impossibility t (R_tid tid)); eauto.
+Qed.
+
+Corollary gcr_ad_invalid_contradiction : forall ad t,
+  gcr t (R_ad ad) = R_invalid ->
+  False.
+Proof.
+  intros. eapply (gcr_invalid_impossibility t (R_ad ad)); eauto.
+Qed.
+
